caseStudy/synthetic/analysisByF/breakConstBT.dfy
@@ -1,21 +1,25 @@
-include "../../../theory/ComplexityNat.dfy"
-include "../../../theory/LemComplexityNat.dfy"
+include "../../../theory/math/LemFunction.dfy"
+include "../../../theory/math/TypeR0.dfy"
+include "../../../theory/ComplexityR0.dfy"
+include "../../../theory/LemComplexityR0.dfy"
 
-import opened ComplexityNat
-import opened LemComplexityNat
+import opened LemFunction
+import opened TypeR0
+import opened ComplexityR0
+import opened LemComplexityR0
 
 type Input {
   function size() : nat
 }
 
-ghost function f(N:nat) : nat
+ghost function f(n:nat) : nat
 {
   1
 }
 
 method breakConstBT(x:Input, P:nat->bool) returns (ghost t:nat)
   ensures t <= f(x.size()) 
-  ensures tIsBigO(x.size(), t, constGrowth())
+  ensures tIsBigO(x.size(), t as R0, constGrowth())
 {
   var N := x.size();
   assume {:axiom} N > 0 ==> P(0);  // best case
@@ -34,5 +38,9 @@ method breakConstBT(x:Input, P:nat->bool) returns (ghost t:nat)
     t := t+1 ;
   }
   assert t <= f(N);
-  assert f in O(constGrowth()) by { lem_bigO_constGrowth(f, 1); }
+  assert liftToR0(f) in O(constGrowth()) by { 
+    lem_bigO_constGrowth(n => 1 as R0, 1.0);
+    lem_fun_Ext(liftToR0(f), n => 1 as R0)
+      by { assert 1 as R0 == 1.0; } 
+  }
 } 
