caseStudy/synthetic/analysisBySum/lin3.dfy
@@ -1,33 +1,36 @@
-include "../../../theory/math/ExpNat.dfy"
+include "../../../theory/math/LemFunction.dfy"
 include "../../../theory/math/SumInt.dfy"
-include "../../../theory/ComplexityNat.dfy"
+include "../../../theory/math/TypeR0.dfy"
+include "../../../theory/ComplexityR0.dfy"
 
-import opened ExpNat
+import opened LemFunction
 import opened SumInt
-import opened ComplexityNat
+import opened TypeR0
+import opened ComplexityR0
 
 type Input {
   function size() : nat
 }
 
-ghost function f(N:nat) : nat
+ghost function f(n:nat) : nat
 {
-  3*exp(N,1)
+  3*n
 }
 
-method lin(x:Input) returns (ghost t:nat, ghost t':nat)
+method lin(x:Input) returns (ghost t:nat)
   ensures t == f(x.size())
-  ensures tIsBigO(x.size(), t, linGrowth())
+  ensures tIsBigO(x.size(), t as R0, linGrowth())
 {
-  var N := x.size();
-  var i, j; reveal sum(); 
-  i, j, t, t' := 0, 0, 0, 0;
+  var N := x.size(); reveal sum(); 
+  t := 0;
+  
+  var i, j := 0, 0;
   while i != 3
       invariant 0 <= i <= 3
       invariant t == sum(1, i, k => sum(1, N, k' => 1))
       decreases 3 - i
   {
-    j := 0; t' := 0;
+    j := 0; ghost var t' := 0;
     while j != N
       invariant 0 <= j <= N
       invariant t' == sum(1, j, k' => 1)
@@ -43,24 +46,21 @@ method lin(x:Input) returns (ghost t:nat, ghost t':nat)
     t := t+t' ;
   }
   assert t == sum(1, 3, k => sum(1, N, k' => 1)); 
-  assert t == f(N) by { reveal exp(); lem_sum_constAll(1, N); }
-  assert t <= f(N);
-  assert f in O(linGrowth()) by { var c, n0 := lem_fBigOlin(); }
+  assert t == f(N) by { lem_sum_constAll(1, N); }
+  assert liftToR0(f) in O(linGrowth()) by { var c, n0 := lem_fBigOlin(); }
 } 
 
-lemma lem_fBigOlin() returns (c:nat, n0:nat)
-  ensures c > 0 && bigOfrom(c, n0, f, linGrowth())
+lemma lem_fBigOlin() returns (c:R0, n0:nat)
+  ensures c > 0.0 && bigOfrom(c, n0, liftToR0(f), linGrowth())
 {
-  c, n0 := 3, 0;
+  c, n0 := 3.0, 0;
   forall n:nat | 0 <= n0 <= n
-    ensures f(n) <= c*linGrowth()(n)
+    ensures f(n) as R0 <= c*linGrowth()(n)
   {
     calc {
-         f(n);
-      == 3*exp(n,1);
-      == { reveal exp(); }
-         3*n;   
+         f(n) as R0;
+      == (3*n) as R0;
+      == c*linGrowth()(n);  
     }
-    assert f(n) <= c*linGrowth()(n); 
   }
 }
