caseStudy/synthetic/analysisBySum/linBefore.dfy
@@ -1,26 +1,28 @@
-include "../../../theory/math/ExpNat.dfy"
+include "../../../theory/math/LemFunction.dfy"
 include "../../../theory/math/SumInt.dfy"
-include "../../../theory/ComplexityNat.dfy"
+include "../../../theory/math/TypeR0.dfy"
+include "../../../theory/ComplexityR0.dfy"
 
-import opened ExpNat
+import opened LemFunction
 import opened SumInt
-import opened ComplexityNat
+import opened TypeR0
+import opened ComplexityR0
 
 type Input {
   function size() : nat
 }
 
-ghost function f(N:nat) : nat
+ghost function f(n:nat) : nat
 {
-  if N < 10 then exp(N,1) else 20
+  if n < 10 then n else 20
 }
 
 method linAfter(x:Input) returns (ghost t:nat)
   ensures t == f(x.size())
-  ensures tIsBigO(x.size(), t, constGrowth())
+  ensures tIsBigO(x.size(), t as R0, constGrowth())
 {
-  var N := x.size();
-  reveal sum();
+  var N := x.size(); reveal sum();
+
   if N < 10 {
     var i;
     i, t := 0, 0;
@@ -38,25 +40,25 @@ method linAfter(x:Input) returns (ghost t:nat)
     // Op. interesante ocurre 20 veces
     t := 20 ;
   }
+
   assert t == if N < 10 then sum(1, N, k => 1) else 20; 
-  assert t == f(N) by { reveal exp(); lem_sum_constAll(1, N); }
-  assert t <= f(N);
-  assert f in O(constGrowth()) by { var c, n0 := lem_fBigOconst(); }
+  assert t == f(N) by { lem_sum_constAll(1, N); }
+  assert liftToR0(f) in O(constGrowth()) by { var c, n0 := lem_fBigOconst(); }
 } 
 
-lemma lem_fBigOconst() returns (c:nat, n0:nat)
-  ensures c > 0 && bigOfrom(c, n0, f, constGrowth())
+lemma lem_fBigOconst() returns (c:R0, n0:nat)
+  ensures c > 0.0 && bigOfrom(c, n0, liftToR0(f), constGrowth())
 {
-  c, n0 := 20, 10; 
+  c, n0 := 20.0, 10; 
   forall n:nat | 0 <= n0 <= n
-    ensures f(n) <= c*constGrowth()(n)
+    ensures f(n) as R0 <= c*constGrowth()(n)
   {
     calc {
-         f(n);
-      == if n < 10 then exp(n,1) else 20;
-      == { reveal exp(); }
-         if n < 10 then n else 20;    
+         f(n) as R0;
+      == (if n < 10 then n else 20) as R0;
+      == 20 as R0;
+      <= c * 1 as R0;
+      == c*constGrowth()(n); 
     }
-    assert f(n) <= c*constGrowth()(n);
   }
 }
