test/testComplexity.dfy
@@ -1,0 +1,83 @@
+include "../theory/math/ExpNat.dfy"
+include "../theory/math/ExpReal.dfy"
+include "../theory/math/LemBoundsNat.dfy"
+include "../theory/math/LemFunction.dfy"
+include "../theory/math/Log2Nat.dfy"
+include "../theory/math/SumInt.dfy"
+include "../theory/math/TypeR0.dfy"
+include "../theory/ComplexityR0.dfy"
+include "../theory/LemComplexityR0.dfy"
+
+import EN = ExpNat
+import opened ExpReal
+import opened LemBoundsNat
+import opened LemFunction
+import opened Log2Nat
+import opened SumInt
+import opened TypeR0
+import opened ComplexityR0
+import opened LemComplexityR0
+
+lemma test_bigOprod()
+  requires liftToR0(n => 2*n) in O(linGrowth())
+  requires liftToR0(n => 3*n) in O(linGrowth())
+  ensures  liftToR0(n => (2*n)*(3*n)) in O(quadGrowth())
+{
+  var f1:nat->R0 := liftToR0(n => 2*n);
+  var f2:nat->R0 := liftToR0(n => 3*n);
+
+  lem_bigO_prod(f1, linGrowth(), f2, linGrowth());  
+  assert (n => f1(n)*f2(n)) in O(n => linGrowth()(n)*linGrowth()(n));
+
+  lem_fun_Ext(n => linGrowth()(n)*linGrowth()(n), quadGrowth())
+    by { lem_fun_EtaApp(linGrowth()); 
+         lem_fun_EtaApp(quadGrowth());
+         forall n:nat ensures (n => linGrowth()(n)*linGrowth()(n))(n) == quadGrowth()(n) { } 
+    }
+  lem_fun_Ext(n => f1(n)*f2(n), liftToR0(n => (2*n)*(3*n))) 
+    by { lem_fun_EtaApp(f1); lem_fun_EtaApp(f2); assert 2.0 == 2 as R0; assert 3.0 == 3 as R0; } 
+}
+
+lemma test_polyBigO() returns (c:R0, n0:nat) 
+  ensures ((n:nat) => 3.0*exp(n as R0,2.0) + 100.0*exp(n as R0,1.0) + 10.0) in O(quadGrowth())
+{
+  var poly := ((n:nat) => 3.0*exp(n as R0,2.0) + 100.0*exp(n as R0,1.0) + 10.0);
+
+  c, n0 := 113.0, 1;
+  forall n:nat | 0 <= n0 <= n
+    ensures poly(n) <= c*quadGrowth()(n)
+  {
+    calc {
+         poly(n);
+      == (3.0*exp(n as R0,2.0) + 100.0*exp(n as R0,1.0) + 10.0) as R0;
+      == { lem_exp_Pow0(n as R0); }
+         (3.0*exp(n as R0,2.0) + 100.0*exp(n as R0,1.0) + 10.0*exp(n as R0,0.0)) as R0;
+      <= { lem_exp_MonoIncr(n as R0, 1.0, 2.0); lem_exp_MonoIncr(n as R0, 0.0, 2.0);  }
+         (3.0*exp(n as R0,2.0) + 100.0*exp(n as R0,2.0) + 10.0*exp(n as R0,2.0)) as R0;
+      == ((3.0 + 100.0 + 10.0)*exp(n as R0,2.0)) as R0;
+      == c*exp(n as R0,2.0) as R0; 
+      == { lem_exp_Pow2(n as R0); }
+         c * (n*n) as R0; 
+    }
+  }
+  assert c > 0.0 && bigOfrom(c, n0, poly, quadGrowth());
+} 
+
+// lemma test_log2BigOlin() returns (c:nat, n0:nat)
+//   ensures ((n:nat) => log2(n+1)) in O(linGrowth())
+// {
+//   c, n0 := 1, 1;
+//   forall n:nat | 0 <= n0 <= n
+//     ensures log2(n+1) <= c*linGrowth()(n)
+//   {
+//     calc {
+//          log2(n+1);
+//       <= { lem_log2nPlus1LEQn(n); }
+//          n;
+//       == { reveal exp(); }
+//          c*exp(n,1);  
+//     }
+//     assert log2(n+1) <= c*linGrowth()(n);
+//   }
+//   assert bigOfrom(c, n0, n => log2(n+1), linGrowth());
+// } 
